High-level proof sketch for the request/response-down cases

src/RqRsCorrect.v
@@ -5,7 +5,7 @@ Require Import Serial SerialFacts.
 Require Import Reduction Commutativity QuasiSeq Topology.
 Require Import RqRsTopo RqRsFacts.
 Require Import RqRsInvMsg RqRsInvLock RqRsInvAtomic.
-Require Import RqRsRed RqUpRed RsUpRed RqDownRed.
+Require Import RqRsRed RqUpRed RsUpRed RqDownRed RsDownRed.
 
 Set Implicit Arguments.
 
@@ -161,57 +161,6 @@ Section Pushable.
     Qed.
 
   End RsUp.
-
-  (** Generally we need to prove:
-   * a) [oinds(hst1) -*- oinds(hst2) -> Reducible (hst2 ++ hst1) (hst1 ++ hst2)]
-   *
-   ** Proof sketch for the reducibility of downward-request labels:
-   * 1) [phst] ⊆ tr(nlbl)^{-1}
-   * 2) Let [olast(hst)] be the last object index of an [Atomic] history [hst].
-   * 2-1) [olast(hst) ∈ tr(nlbl) -> oinds(hst) ⊆ tr(nlbl)]
-   * 2-2) [olast(hst) ∈ tr(nlbl)^{-1} -> 
-   *       exists preh posth, 
-   *         hst = posth ++ preh /\
-   *         ("preh" just consists of RqUp labels) /\
-   *         oinds(posth) ⊆ tr(nlbl)^{-1}]
-   * 3) Now define [LPush] and [RPush] as follows:
-   *    [LPush hst ≜ olast(hst) ∈ tr(nlbl)]
-   *    [RPush hst ≜ olast(hst) ∈ tr(nlbl)^{-1}]
-   * 4) To check each condition in [PushableHst]:
-   * 4-1) Left-or-right: [olast(hst)] is a single object index, 
-   *      thus [in_dec eq_nat_dec olast(hst) tr(nlbl)] provides enough
-   *      information.
-   * 4-2) Left-push-reducibility: if [hst] is left-pushable, then by 2-1) and 3)
-   *      we get [oinds(hst) ⊆ tr(nlbl)]. Now by 1) and a) we exactly get the
-   *      reducibility.
-   * 4-3) Right-push-reducibility: if [hst] is right-pushable, then by 2-2) 
-   *      and 3) we have [preh] and [posth] that satisfy the conditions in 2-2).
-   * 4-3-1) [preh] and [nlbl] are commutative since [preh] only consists of 
-   *        RqUp labels.
-   * 4-3-2) [posth] and [nlbl] are commutative by applying a).
-   * 4-4) [LRPushable]: if [RPush hst1 /\ LPush hst2], then by 2-1), 2-2), 
-   *      and 3) for [hst1] we have [preh1] and [posth1] that satisfy the
-   *      conditions in 2-2). Now reasoning very similarly to 4-2) and 4-3):
-   * 4-4-1) [preh1] and [hst2] are commutative since [preh1] only consists of
-   *        RqUp labels.
-   * 4-4-2) [posth1] and [hst2] are commutative by applying a).
-   *
-   ** Proof sketch for the reducibility of downward-response labels:
-   * 1) [exists preh posth, 
-   *       phst = posth ++ preh /\
-   *       ("preh" just consists of RqUp labels) /\
-   *       oinds(posth) ⊆ tr(nlbl)^{-1}]
-   * 2) Let [olast(hst)] be the last object index of an [Atomic] history [hst].
-   * 2-1) [olast(hst) ∈ tr(nlbl) -> oinds(hst) ⊆ tr(nlbl)]
-   * 2-2) [olast(hst) ∈ tr(nlbl)^{-1} -> oinds(hst) ⊆ tr(nlbl)^{-1}]
-   *      This part differs from the one for downward-requests since both upward
-   *      requests and upward responses cannot happen when a downward-response label is
-   *      in the message pool.
-   * 3) Define [LPush] and [RPush] as follows:
-   *    [LPush hst ≜ olast(hst) ∈ tr(nlbl)]
-   *    [RPush hst ≜ olast(hst) ∈ tr(nlbl)^{-1}]
-   * 4) Conditions of [PushableHst] are easier to prove, mostly by a).
-   *)
 
   Section RqDown.
     Hypothesis (Hrd: RqDownMsgs dtr oidx rins).
@@ -412,8 +361,238 @@ Section Pushable.
       destruct H10.
       eapply rqDown_LRPushable_unit_reducible; try eassumption.
     Qed.
-    
+
+    Lemma rqDown_WellInterleavedHst:
+      WellInterleavedHst sys phst nlbl.
+    Proof.
+      apply PushableHst_WellInterleavedHst with (P:= RqDownP rins); auto.
+      - eauto using rqDown_PInitializing.
+      - exists RqDownLPush, RqDownRPush.
+        intros; repeat split.
+        + eauto using rqDown_PPreserving.
+        + eauto using rqDown_lpush_or_rpush.
+        + eauto using rqDown_lpush_reducible.
+        + eauto using rqDown_rpush_reducible.
+        + eauto using rqDown_LRPushable.
+    Qed.
+
   End RqDown.
+
+  Section RsDown.
+    Hypothesis (Hrd: RsDownMsgs dtr oidx rins).
+
+    Definition RsDownLPush (hst: MHistory) :=
+      exists loidx,
+        lastOIdxOf hst = Some loidx /\
+        In loidx (subtreeIndsOf dtr oidx).
+
+    Definition RsDownRPush (hst: MHistory) :=
+      exists loidx,
+        lastOIdxOf hst = Some loidx /\
+        ~ In loidx (subtreeIndsOf dtr oidx).
+
+    Lemma rsDown_PInitializing:
+      PInitializing sys (RsDownP rins) phst.
+    Proof.
+      intros; red; intros.
+      destruct Hcont as [eouts [oidx' [ridx' [rins' [routs' ?]]]]]; dest.
+      apply eq_sym in H1; inv H1.
+      inv H0.
+      red; eapply SubList_forall; [|eassumption].
+      eapply (atomic_messages_eouts_in msg_dec); eauto.
+    Qed.
+
+    Lemma rsDown_discontinuous_PPreserving:
+      forall hst,
+        Discontinuous phst hst ->
+        PPreserving sys RsUpP hst.
+    Proof.
+      intros.
+      destruct Hcont as [eouts [oidx' [ridx' [rins' [routs' ?]]]]]; dest.
+      apply eq_sym in H1; inv H1.
+
+      inv H0.
+      destruct H as [inits1 [ins1 [outs1 [eouts1 [inits2 [ins2 [outs2 [eouts2 ?]]]]]]]].
+      dest.
+      eapply atomic_unique in H; [|eassumption]; dest; subst.
+
+      red; intros.
+      eapply (atomic_messages_ins_ins msg_dec).
+      - eapply H0.
+      - eassumption.
+      - assumption.
+      - eapply DisjList_comm, DisjList_SubList; eauto.
+    Qed.
+
+    Lemma rsDown_PPreserving:
+      forall st1,
+        Reachable (steps step_m) sys st1 ->
+        forall hsts st2,
+          Forall (AtomicEx msg_dec) hsts ->
+          steps step_m sys st1 (nlbl :: List.concat hsts ++ phst) st2 ->
+          Forall (fun hst => Discontinuous phst hst) hsts ->
+          Forall (PPreserving sys (RsDownP rins)) hsts.
+    Proof.
+      intros.
+      eapply Forall_impl; [|eapply H2].
+      simpl; intros hst ?.
+      eapply rsDown_discontinuous_PPreserving; assumption.
+    Qed.
+
+    Lemma rsDown_lpush_or_rpush:
+      forall st1,
+        Reachable (steps step_m) sys st1 ->
+        forall hsts st2,
+          Forall (AtomicEx msg_dec) hsts ->
+          steps step_m sys st1 (nlbl :: List.concat hsts ++ phst) st2 ->
+          Forall (fun hst => Discontinuous phst hst) hsts ->
+          Forall (fun hst => RsDownLPush hst \/ RsDownRPush hst) hsts.
+    Proof.
+      intros; clear -H0.
+      rewrite Forall_forall in H0.
+      apply Forall_forall.
+      intros hst ?.
+      specialize (H0 _ H).
+      destruct H0 as [inits [ints [outs [eouts ?]]]].
+      apply atomic_lastOIdxOf in H0.
+      destruct H0 as [loidx ?].
+      destruct (in_dec eq_nat_dec loidx (subtreeIndsOf dtr oidx)).
+      - left; red; eauto.
+      - right; red; eauto.
+    Qed.
+
+    Lemma rsDown_lpush_unit:
+      forall hst,
+        AtomicEx msg_dec hst ->
+        Discontinuous phst hst ->
+        RsDownLPush hst ->
+        Reducible sys (hst ++ phst) (phst ++ hst).
+    Proof.
+      intros.
+      destruct Hcont as [peouts [oidx' [ridx' [rins' [routs' ?]]]]]; dest.
+      apply eq_sym in H3; inv H3.
+      inv H2.
+      destruct H0 as [inits1 [ins1 [outs1 [eouts1 ?]]]].
+      destruct H0 as [inits2 [ins2 [outs2 [eouts2 ?]]]]; dest.
+      pose proof (atomic_unique H6 H0); dest; subst; clear H0.
+      destruct H1 as [loidx [? ?]].
+      eapply rsDown_lpush_unit_reducible; eauto.
+      apply rsDown_PInitializing.
+    Qed.
+    
+    Lemma rsDown_lpush_reducible:
+      forall st1,
+        Reachable (steps step_m) sys st1 ->
+        forall hsts st2,
+          Forall (AtomicEx msg_dec) hsts ->
+          steps step_m sys st1 (nlbl :: List.concat hsts ++ phst) st2 ->
+          Forall (fun hst => Discontinuous phst hst) hsts ->
+          Forall (fun hst => RsDownLPush hst ->
+                             Reducible sys (hst ++ phst) (phst ++ hst)) hsts.
+    Proof.
+      intros.
+      inv_steps.
+      eapply steps_split in H6; [|reflexivity].
+      destruct H6 as [sti [? ?]].
+      clear H8.
+      generalize dependent st3.
+      induction hsts as [|hst hsts]; simpl; intros; [constructor|].
+      inv H0; inv H2.
+      eapply steps_split in H3; [|reflexivity].
+      destruct H3 as [hsti [? ?]].
+      specialize (IHhsts H7 H8 _ H0).
+      constructor; [|assumption].
+      intros; apply rsDown_lpush_unit; auto.
+    Qed.
+
+    Lemma rsDown_rpush_unit:
+      forall hst,
+        RsDownRPush hst ->
+        AtomicEx msg_dec hst ->
+        Discontinuous phst hst ->
+        ReducibleP sys (RsDownP rins) (nlbl :: hst) (hst ++ [nlbl]).
+    Proof.
+      intros.
+      destruct H0 as [inits [ins [outs [eouts ?]]]].
+      destruct Hcont as [peouts [oidx' [ridx' [rins' [routs' ?]]]]]; dest.
+      apply eq_sym in H3; inv H3.
+      destruct H2 as [pinits pins phst pouts peouts].
+      red in H1; dest.
+      pose proof (atomic_unique H1 H3); dest; subst; clear H3.
+      pose proof (atomic_unique H6 H0); dest; subst; clear H6.
+      destruct H as [loidx [? ?]].
+      eapply rsDown_rpush_unit_reducible; eauto.
+      eapply DisjList_SubList; eauto.
+    Qed.
+
+    Lemma rsDown_rpush_reducible:
+      forall st1,
+        Reachable (steps step_m) sys st1 ->
+        forall hsts st2,
+          Forall (AtomicEx msg_dec) hsts ->
+          steps step_m sys st1 (nlbl :: List.concat hsts ++ phst) st2 ->
+          Forall (fun hst => Discontinuous phst hst) hsts ->
+          Forall (fun hst => RsDownRPush hst ->
+                             ReducibleP sys (RsDownP rins) (nlbl :: hst) (hst ++ [nlbl])) hsts.
+    Proof.
+      intros.
+      clear H1.
+      induction hsts as [|hst hsts]; simpl; intros; [constructor|].
+      inv H0; inv H2.
+      constructor; eauto.
+      intros; eapply rsDown_rpush_unit; eauto.
+    Qed.
+
+    Lemma rsDown_LRPushable:
+      forall st1,
+        Reachable (steps step_m) sys st1 ->
+        forall hsts st2,
+          Forall (AtomicEx msg_dec) hsts ->
+          steps step_m sys st1 (nlbl :: List.concat hsts ++ phst) st2 ->
+          Forall (fun hst => Discontinuous phst hst) hsts ->
+          LRPushable sys (RsDownP rins) RsDownLPush RsDownRPush hsts.
+    Proof.
+      intros; red; intros; subst.
+      apply Forall_app_inv in H0; dest.
+      inv H3; destruct H8 as [inits1 [ins1 [outs1 [eouts1 ?]]]].
+      apply Forall_app_inv in H9; dest.
+      inv H7; destruct H10 as [inits2 [ins2 [outs2 [eouts2 ?]]]].
+      destruct H4 as [lloidx [? ?]].
+      destruct H5 as [rloidx [? ?]].
+
+      assert (DisjList rins inits1 /\ DisjList rins inits2).
+      { destruct Hcont as [peouts [oidx' [ridx' [rins' [routs' ?]]]]]; dest.
+        apply eq_sym in H12; inv H12.
+        apply Forall_app_inv in H2; dest.
+        inv H12; apply Forall_app_inv in H18; dest.
+        inv H15.
+        red in H17, H19; dest.
+        pose proof (atomic_unique H19 H3); dest; subst; clear H19.
+        pose proof (atomic_unique H16 H7); dest; subst; clear H16.
+        inv H10.
+        pose proof (atomic_unique H17 H19); dest; subst; clear H17.
+        pose proof (atomic_unique H15 H19); dest; subst; clear H15.
+        split; eapply DisjList_SubList; eassumption.
+      }
+      destruct H10.
+      eapply rsDown_LRPushable_unit_reducible; try eassumption.
+    Qed.
+
+    Lemma rsDown_WellInterleavedHst:
+      WellInterleavedHst sys phst nlbl.
+    Proof.
+      apply PushableHst_WellInterleavedHst with (P:= RqDownP rins); auto.
+      - eauto using rsDown_PInitializing.
+      - exists RqDownLPush, RqDownRPush.
+        intros; repeat split.
+        + eauto using rsDown_PPreserving.
+        + eauto using rsDown_lpush_or_rpush.
+        + eauto using rsDown_lpush_reducible.
+        + eauto using rsDown_rpush_reducible.
+        + eauto using rsDown_LRPushable.
+    Qed.
+    
+  End RsDown.
   
 End Pushable.
 
@@ -441,22 +620,11 @@ Proof.
   destruct Hnlbl as [oidx [ridx [rins [routs ?]]]]; dest; subst.
 
   destruct H6 as [|[|[|]]].
-  - apply LPushableHst_WellInterleavedHst; auto.
-    eauto using rqUp_LPushableHst.
-  - apply PushableHst_WellInterleavedHst with (P:= RqDownP rins); auto.
-    + eauto using rqDown_PInitializing.
-    + exists (RqDownLPush dtr oidx), (RqDownRPush dtr oidx).
-      intros; repeat split.
-      * eauto using rqDown_PPreserving.
-      * eauto using rqDown_lpush_or_rpush.
-      * eauto using rqDown_lpush_reducible.
-      * eauto using rqDown_rpush_reducible.
-      * eauto using rqDown_LRPushable.
-  - apply RPushableHst_WellInterleavedHst with (P:= RsUpP rins); auto.
-    + eauto using rsUp_PInitializing.
-    + eauto using rsUp_RPushableHst.
-  - admit.
-Admitted.
+  - eapply rqUp_WellInterleavedHst; eauto.
+  - eapply rqDown_WellInterleavedHst; eauto.
+  - eapply rsUp_WellInterleavedHst; eauto.
+  - eapply rsDown_WellInterleavedHst; eauto.
+Qed.
 
 Corollary rqrs_Serializable:
   forall {oifc} (sys: System oifc) (dtr: DTree),
