src/RsDownRed.v
@@ -1,0 +1,220 @@
+Require Import Peano_dec Omega List ListSupport.
+Require Import Common FMap.
+Require Import Syntax Semantics SemFacts StepM Invariant.
+Require Import Serial SerialFacts.
+Require Import Reduction Commutativity QuasiSeq Topology.
+Require Import RqRsTopo RqRsFacts.
+Require Import RqRsInvMsg RqRsInvLock RqRsInvAtomic.
+Require Import RqUpRed RsUpRed RqRsRed.
+
+Set Implicit Arguments.
+
+Open Scope list.
+Open Scope fmap.
+
+(** Proof sketch for the reducibility of downward-response labels:
+ * 1) [exists preh posth, 
+ *       phst = posth ++ preh /\
+ *       ("preh" just consists of RqUp labels) /\
+ *       oinds(posth) ⊆ tr(nlbl)^{-1}]
+ * 2) Let [olast(hst)] be the last object index of an [Atomic] history [hst].
+ * 2-1) [olast(hst) ∈ tr(nlbl) -> oinds(hst) ⊆ tr(nlbl)]
+ * 2-2) [olast(hst) ∈ tr(nlbl)^{-1} -> oinds(hst) ⊆ tr(nlbl)^{-1}]
+ *      This part differs from the one for downward-requests since both upward
+ *      requests and upward responses cannot happen when a downward-response label is
+ *      in the message pool.
+ * 3) Define [LPush] and [RPush] as follows:
+ *    [LPush hst ≜ olast(hst) ∈ tr(nlbl)]
+ *    [RPush hst ≜ olast(hst) ∈ tr(nlbl)^{-1}]
+ * 4) Conditions of [PushableHst] are easier to prove, mostly by a).
+ *)
+
+Section RsDownReduction.
+  Context {oifc: OStateIfc}.
+  Variables (dtr: DTree)
+            (sys: System oifc).
+
+  Hypothesis (Hrrs: RqRsSys dtr sys).
+
+  Section OnRsDown.
+    Variables (oidxTo: IdxT)
+              (rsDowns: list (Id Msg)).
+    Hypothesis (Hrsd: RsDownMsgs dtr oidxTo rsDowns).
+
+    Lemma rsDown_oinds:
+      forall inits ins hst outs eouts,
+        SubList rsDowns eouts ->
+        Atomic msg_dec inits ins hst outs eouts ->
+        forall st1 st2,
+          Reachable (steps step_m) sys st1 ->
+          steps step_m sys st1 hst st2 ->
+          exists phst ruIdx rqUps ninits nins nhst nouts,
+            hst = nhst ++ phst /\
+            (phst = nil \/
+             (RqUpMsgs dtr ruIdx rqUps /\ RqUpHistory dtr phst rqUps)) /\
+            SubList (oindsOf phst) (subtreeIndsOf dtr oidxTo) /\
+            SubList ninits ins /\
+            Atomic msg_dec ninits nins nhst nouts eouts /\
+            DisjList (oindsOf nhst) (subtreeIndsOf dtr oidxTo).
+    Proof.
+    Admitted.
+
+    Lemma rsDown_olast_inside_tree:
+      forall inits ins hst outs eouts,
+        DisjList rsDowns inits ->
+        Atomic msg_dec inits ins hst outs eouts ->
+        forall st1 st2 loidx,
+          Reachable (steps step_m) sys st1 ->
+          Forall (InMPI st1.(bst_msgs)) rsDowns ->
+          steps step_m sys st1 hst st2 ->
+          lastOIdxOf hst = Some loidx ->
+          In loidx (subtreeIndsOf dtr oidxTo) ->
+          SubList (oindsOf hst) (subtreeIndsOf dtr oidxTo).
+    Proof.
+    Admitted.
+
+    Lemma rsDown_olast_outside_tree:
+      forall inits ins hst outs eouts,
+        DisjList rsDowns inits ->
+        Atomic msg_dec inits ins hst outs eouts ->
+        forall st1 st2 loidx,
+          Reachable (steps step_m) sys st1 ->
+          Forall (InMPI st1.(bst_msgs)) rsDowns ->
+          steps step_m sys st1 hst st2 ->
+          lastOIdxOf hst = Some loidx ->
+          ~ In loidx (subtreeIndsOf dtr oidxTo) ->
+          DisjList (oindsOf hst) (subtreeIndsOf dtr oidxTo).
+    Proof.
+    Admitted.
+
+    Definition RsDownP (st: MState oifc) :=
+      Forall (InMPI st.(bst_msgs)) rsDowns.
+
+    Lemma rsDown_lpush_rpush_unit_reducible:
+      forall rinits rins rhst routs reouts
+             linits lins lhst louts leouts,
+        Atomic msg_dec rinits rins rhst routs reouts ->
+        DisjList (oindsOf rhst) (subtreeIndsOf dtr oidxTo) ->
+        Atomic msg_dec linits lins lhst louts leouts ->
+        SubList (oindsOf lhst) (subtreeIndsOf dtr oidxTo) ->
+        DisjList reouts linits ->
+        Reducible sys (lhst ++ rhst) (rhst ++ lhst).
+    Proof.
+      intros.
+      eapply rqrs_reducible; try eassumption.
+      eapply DisjList_comm, DisjList_SubList; [eassumption|].
+      apply DisjList_comm; assumption.
+    Qed.
+    
+    Lemma rsDown_lpush_unit_reducible:
+      forall pinits pins phst pouts peouts
+             inits ins hst outs eouts loidx,
+        PInitializing sys RsDownP phst ->
+        Atomic msg_dec pinits pins phst pouts peouts ->
+        SubList rsDowns peouts ->
+        Atomic msg_dec inits ins hst outs eouts ->
+        lastOIdxOf hst = Some loidx ->
+        In loidx (subtreeIndsOf dtr oidxTo) ->
+        DisjList peouts inits ->
+        Reducible sys (hst ++ phst) (phst ++ hst).
+    Proof.
+      intros; red; intros.
+      eapply steps_split in H6; [|reflexivity].
+      destruct H6 as [sti [? ?]].
+
+      pose proof (rsDown_oinds H1 H0 Hr H6).
+      destruct H8 as [pphst [ruIdx [rqUps [ninits [nins [nphst [nouts ?]]]]]]].
+      dest; subst.
+      eapply steps_split in H6; [|reflexivity].
+      destruct H6 as [psti [? ?]].
+
+      rewrite <-app_assoc.
+      eapply reducible_app_1; try assumption.
+      - instantiate (1:= hst ++ pphst).
+        destruct H9; dest; subst; simpl in *.
+        + rewrite app_nil_r; apply reducible_refl.
+        + eapply rqUpHistory_lpush_unit_reducible; eauto.
+          admit.
+      - rewrite app_assoc.
+        eapply reducible_app_2; try assumption.
+        + instantiate (1:= hst ++ nphst).
+          eapply rsDown_lpush_rpush_unit_reducible; try eassumption.
+          eapply rsDown_olast_inside_tree.
+          * eapply DisjList_SubList; eassumption.
+          * eassumption.
+          * eapply reachable_steps; [eassumption|].
+            eapply steps_append; eassumption.
+          * eapply H.
+            eapply steps_append; eassumption.
+          * eassumption.
+          * eassumption.
+          * eassumption.
+        + rewrite <-app_assoc.
+          eapply steps_append; [|eassumption].
+          eapply steps_append; eassumption.
+    Admitted.
+
+    Lemma rsDown_rpush_unit_reducible:
+      forall inits ins hst outs eouts loidx ridx routs,
+        Atomic msg_dec inits ins hst outs eouts ->
+        lastOIdxOf hst = Some loidx ->
+        ~ In loidx (subtreeIndsOf dtr oidxTo) ->
+        DisjList rsDowns inits ->
+        ReducibleP sys RsDownP (RlblInt oidxTo ridx rsDowns routs :: hst)
+                   (hst ++ [RlblInt oidxTo ridx rsDowns routs]).
+    Proof.
+      intros; red; intros.
+      inv_steps.
+      eapply rsDown_lpush_rpush_unit_reducible; try eassumption.
+      - eapply rsDown_olast_outside_tree; eassumption.
+      - constructor.
+      - simpl.
+        (* [In oidxTo (subtreeIndsOf dtr oidxTo)] when [oidxTo] is valid. *)
+        admit.
+      - (* For an [Atomic] history, 
+         * if [DisjList rqDowns inits] then [DisjList eouts rqDowns] *)
+        admit.
+      - simpl; econstructor; eassumption.
+    Admitted.
+
+    Lemma rsDown_LRPushable_unit_reducible:
+      forall rinits rins rhst routs reouts rloidx
+             linits lins lhst louts leouts lloidx,
+        Atomic msg_dec rinits rins rhst routs reouts ->
+        DisjList rsDowns rinits ->
+        lastOIdxOf rhst = Some rloidx ->
+        ~ In rloidx (subtreeIndsOf dtr oidxTo) ->
+        Atomic msg_dec linits lins lhst louts leouts ->
+        DisjList rsDowns linits ->
+        lastOIdxOf lhst = Some lloidx ->
+        In lloidx (subtreeIndsOf dtr oidxTo) ->
+        ReducibleP sys RsDownP (lhst ++ rhst) (rhst ++ lhst).
+    Proof.
+      intros; red; intros.
+      eapply steps_split in H7; [|reflexivity].
+      destruct H7 as [sti [? ?]].
+
+      eapply rsDown_olast_inside_tree in H6;
+        [|exact H4
+         |eassumption
+         |eapply reachable_steps; eassumption
+         |eapply (atomic_messages_ins_ins msg_dec);
+          try eapply H; try eassumption;
+          apply DisjList_comm; assumption
+         |eassumption
+         |eassumption].
+      clear H5.
+
+      eapply rsDown_olast_outside_tree in H2;
+        try exact H0; try eassumption.
+      clear H1.
+
+      eapply rsDown_lpush_rpush_unit_reducible; try eassumption.
+      - admit.
+      - eapply steps_append; eassumption.
+    Admitted.
+    
+  End OnRsDown.
+
+End RsDownReduction.
+
